---
tags:
  - exercise
  - math/abstract_algebra
related topics:
  - "[[Isomorphism]]"
  - "[[Group|Trivial group]]"
---
Let $G$, $H$ be groups, and assume that $G \cong H \times G$. Can you conclude that $H$
is trivial? (Hint: No. Can you construct a counterexample?)
##### Solution:
Let $G=(\mathbb{Z}[x],+)$ and $H=(\mathbb{Z},+)$. Consider the functions$$
\begin{align}
  \begin{aligned}
    \phi : \mathbb{Z}[x] &\to \mathbb{Z} \times \mathbb{Z}[x]\\
    \sum_{i=0}^n a_i x^i &\mapsto \left(a_0, \sum_{i=1}^n a_i x^{i-1}\right)
  \end{aligned}\qquad
  \begin{aligned}
    \psi : \mathbb{Z} \times \mathbb{Z}[x] &\to \mathbb{Z}[x]\\
    \left(p, \sum_{i=0}^n a_i x^i\right) &\mapsto p + \sum_{i=0}^n a_i x^{i+1}
  \end{aligned}
\end{align}
$$
- $\phi$ is an homomorphism:
  Let $A,B\in \mathbb{Z}[x]$ with $A=\sum_{i=0}^n a_i x^i$ and $B=\sum_{i=0}^m b_i x^i$. Let $a_i=0$ for $i>n$ and $b_i=0$ for $i>m$, then$$
  \begin{align}
    \phi(A+B)
    &= \phi\left(\sum_{i=0}^n a_i x^i + \sum_{i=0}^m b_i x^i\right)\\
    &= \phi\left(\sum_{i=0}^{\max(n,m)} a_i x^i + \sum_{i=0}^{\max(n,m)} b_i x^i\right)\\
    &= \phi\left(\sum_{i=0}^{\max(n,m)} (a_i + b_i) x^i\right)\\
    &= \left(a_0 + b_0, \sum_{i=1}^{\max(n,m)} (a_i + b_i) x^{i-1}\right)\\
    &= \left(a_0 + b_0, \sum_{i=1}^{\max(n,m)} a_i x^{i-1} + \sum_{i=1}^{\max(n,m)} b_i x^{i-1}\right)\\
    &= \left(a_0 + b_0, \sum_{i=1}^{n} a_i x^{i-1} + \sum_{i=1}^{m} b_i x^{i-1}\right)\\
    &= \left(a_0, \sum_{i=1}^{n} a_i x^{i-1}\right) + \left(b_0, \sum_{i=1}^{m} b_i x^{i-1}\right)\\
    &= \phi\left(\sum_{i=0}^{n} a_i x^{i}\right) + \phi\left(\sum_{i=0}^{n} a_i x^{i}\right)\\
    &= \phi(A) + \phi(B)
  \end{align}
  $$so $\phi$ is an homomorphism.
- $\psi$ is an homomorphism:
  Let $A,B\in \mathbb{Z}\times\mathbb{Z}[x]$ with $A=\left(p,\sum_{i=0}^n a_i x^i\right)$ and $B=\left(q,\sum_{i=0}^m b_i x^i\right)$. Let $a_i=0$ for $i>n$ and $b_i=0$ for $i>m$, then$$
  \begin{align}
    \psi(A+B)
    &= \psi\left(\left(p, \sum_{i=0}^n a_i x^i\right) + \left(q, \sum_{i=0}^m b_i x^i\right)\right)\\
    &= \psi\left(p+q, \sum_{i=0}^{n} a_i x^i + \sum_{i=0}^{m} b_i x^i\right)\\
    &= \psi\left(p+q, \sum_{i=0}^{\max(n,m)} a_i x^i + \sum_{i=0}^{\max(n,m)} b_i x^i\right)\\
    &= \psi\left(p+q, \sum_{i=0}^{\max(n,m)} (a_i + b_i) x^i\right)\\
    &= p+q + \sum_{i=0}^{\max(n,m)} (a_i + b_i) x^{i+1}\\
    &= p + \sum_{i=0}^{\max(n,m)} a_i x^{i+1} + q + \sum_{i=0}^{\max(n,m)} b_i x^{i+1}\\
    &= p + \sum_{i=0}^{n} a_i x^{i+1} + q + \sum_{i=0}^{m} b_i x^{i+1}\\
    &= \psi\left(p, \sum_{i=0}^{n} a_i x^{i}\right) + \psi\left(q, \sum_{i=0}^{m} b_i x^{i}\right)\\
    &= \psi(A) + \psi(B)
  \end{align}
  $$so $\psi$ is an homomorphism.
- $\phi\psi = \text{id}_\mathbb{Z}$:
  Let $A\in \mathbb{Z}[x]$ with $A=\sum_{i=0}^n a_i x^i$, then
  $$
  \begin{align}
    (A)(\phi\psi)
    &= \left(\sum_{i=0}^n a_i x^i\right)(\phi\psi)\\
    &= \left(a_0, \sum_{i=1}^n a_i x^{i-1}\right)\psi\\
    &= a_0 + \sum_{i=1}^n a_i x^i\\
    &= \sum_{i=0}^n a_i x^i\\
    &= A
  \end{align}
  $$so $\phi\psi = \text{id}_\mathbb{Z}$.
- $\psi\phi = \text{id}_{\mathbb{Z}\times\mathbb{Z}[x]}$:
  Let $A\in \mathbb{Z}\times\mathbb{Z}[x]$ with $A=\left(p,\sum_{i=0}^n a_i x^i\right)$, then
  $$
  \begin{align}
    (A)(\psi\phi)
    &= \left(p, \sum_{i=0}^n a_i x^i\right)(\psi\phi)\\
    &= \left(p + \sum_{i=0}^n a_i x^{i+1}\right)\phi\\
    &= \left(p, \sum_{i=0}^n a_i x^i\right)\\
    &= A
  \end{align}
  $$so $\psi\phi = \text{id}_{\mathbb{Z}\times\mathbb{Z}[x]}$.
Then $(\mathbb{Z}[x],+) \cong (\mathbb{Z}\times \mathbb{Z}[x], +)$ in $\mathbf{Grp}$ even though $(\mathbb{Z},+)$ is not trivial.
