---
tags:
  - exercise
  - abstract_algebra
related topics:
  - "[[Abelian group]]"
---
Prove that in a group, $(ab)^2 = a^2 b^2$ if and only if $ab = ba$. Prove that in a group, $(ab)^{−2} = b^{−2}a^{−2}$ if and only if $ab = ba$.
##### Solution:
- $(ab)^2 = a^2 b^2 \iff ab = ba$:
	- $\implies$:$$
		\begin{align}
			(ab)^2 &= a^2 b^2\\
			abab &= a^2 b^2\\
			a^{-1} abab b^{-1} &= a^{-1} a^2 b^2 b^{-1}\\
			ba &= ab
		\end{align}
		$$
	- $\impliedby$:$$
		\begin{align}
			ab &= ba\\
			aabb &= abab\\
			a^2b^2 &= (ab)^2
		\end{align}
		$$
- $(ab)^{−2} = b^{−2}a^{−2} \iff ab = ba$:
	- $\implies$:$$
		\begin{align}
			(ab)^{−2} &= b^{−2}a^{−2}\\
			ab (ab)^{−2} &= ab b^{−2}a^{−2}\\
			(ab)^{-1} &= ab^{-1}a^{-2}\\
			b^{-1} a^{-1} a^2 &= ab^{-1}a^{-2} a^2\\
			b^{-1}a &=ab^{-1}\\
			bb^{-1}ab &=bab^{-1}b\\
			ab &= ba
		\end{align}
		$$
	- $\impliedby$:$$
		\begin{align}
			(ab)^{-2} &= ((ab)^2)^{-1}\\
				&= (abab)^{-1}\\
				&= b^{-1}a^{-1}b^{-1}a^{-1}\\
				&= b^{-1}b^{-1}a^{-1}a^{-1}\\
				&= b^{-2} a^{-2}
		\end{align}
		$$
