---
tags:
  - exercise
  - number_theory
---
Determine
- $51\operatorname{ mod }13$
- $342\operatorname{ mod }85$
- $62\operatorname{ mod }15$
- $10\operatorname{ mod }15$
- $(82\cdot 73)\operatorname{ mod }7$
- $(51+68)\operatorname{ mod }7$
- $(35\cdot 24)\operatorname{ mod }11$
- $(47+68)\operatorname{ mod }11$
##### Solution:
- $51\operatorname{ mod }13$:
	$51 = 3(13) + 12$, so $51\operatorname{ mod }13 = 12$.
- $342\operatorname{ mod }85$:
	$342 = 4(85) + 2$, so $342\operatorname{ mod }85=2$.
- $62\operatorname{ mod }15$:
	$62 = 4(15) + 2$, so $62\operatorname{ mod }15=2$.
- $10\operatorname{ mod }15$:
	$10 = 0(15) + 10$, so $10\operatorname{ mod }15=10$.
- $(82\cdot 73)\operatorname{ mod }7$:
	$82 = 11(7) + 5$, $73=10(7) + 3$, and $15 = 2(7) + 1$ so by [[Mod Distributes Over Multiplication]] $$
	\begin{align}
		(82\cdot 73)\operatorname{ mod }7
		&= (82 \operatorname{ mod } 7)(73 \operatorname{ mod } 7)\operatorname{ mod } 7\\
		&= (5 \cdot 3) \operatorname{ mod } 7\\
		&= 15 \operatorname{ mod } 7\\
		&= 1
	\end{align}
	$$
- $(51+68)\operatorname{ mod }7$:
	$51 = 7(7) + 2$, $68 = 9(7) + 5$, and $7 = 1(7) + 0$, so by [[Mod Distributes Over Addition]]$$
	\begin{align}
		(51+68)\operatorname{ mod }7
		&= \big((51 \operatorname{ mod }7) 
			+ (68\operatorname{mod}7)\big)
			\operatorname{mod}7\\
		&= (2 + 5) \operatorname{mod} 7\\
		&= 7 \operatorname{mod} 7\\
		&= 0
	\end{align}
	$$
- $(35\cdot 24)\operatorname{ mod }11$:
	$35=3(11) + 2$, $24 = 2(11) + 2$, and $4=0(11)+4$, so by [[Mod Distributes Over Multiplication]]$$
	\begin{align}
		(35\cdot 24)\operatorname{ mod }11
		&= (35\operatorname{mod}11)
			(24\operatorname{mod}11)
			\operatorname{ mod }11\\
		&= (2\cdot 2)\operatorname{ mod }11\\
		&= 4 \operatorname{ mod }11\\
		&= 4
	\end{align}
	$$
- $(47+68)\operatorname{ mod }11$:
	$47 = 4(11) + 3$, $68 = 6(11) + 2$, and $5 = 0(11) + 5$, so by [[Mod Distributes Over Addition]]$$
	\begin{align}
		(47+68)\operatorname{ mod }11
		&= \big((47\operatorname{mod}11)+(68\operatorname{mod}11)\big)\operatorname{ mod }11\\
		&= (3 + 2)\operatorname{ mod }11\\
		&= 5 \operatorname{ mod }11\\
		&= 5
	\end{align}
	$$