---
tags:
  - exercise
  - math/abstract_algebra
related topics:
  - "[[Group]]"
---
If $a_1, a_2,\dots , a_n$ belong to a group, what is the inverse of $a_1 a_2\dots a_n$?
##### Solution:
Lets prove by induction that $(a_1 a_2\dots a_n)^{-1}=a_n^{-1}\dots a_2^{-1} a_1^{-1}$
- Step $n=1$:
	$a_1^{-1} = a_1^{-1}$.
- Step $n+1$:$$
	
		(a_1 a_2\dots a_n a_{n+1})^{-1}
		&= \left((a_1 a_2\dots a_n) a_{n+1}\right)^{-1}\
		&= a_{n+1}^{-1} (a_1 a_2\dots a_n)^{-1}\tag{$*$}\
		&= a_{n+1}^{-1} a_n^{-1}\dots a_2^{-1} a_1^{-1}
			&\text{by induction}
	
	$$Where ($*$) is by [[Socks-shoes property]].
The property then holds for all $n$.